remove old files

code/rocq/det.v
@@ -1,3 +1,4 @@
+(* Require Import Coq.Program.Wf. *)
 From mathcomp Require Import all_ssreflect.
 
 Inductive D := Func | Pred.
@@ -10,7 +11,10 @@ Notation "x '--o-->' y" := (arr o x y) (at level 3).
 Definition P := nat.
 Definition K := nat.
 Definition V := nat.
-Inductive C := p of P | v of V.
+Inductive C := 
+  | p of P 
+  | v of V
+  .
 Inductive Tm := 
   | Code : C -> Tm
   | Data : K -> Tm
@@ -19,8 +23,8 @@ Inductive Tm :=
 Record R_ {A} := { pred : P; args : list Tm; premises : list A }.
 Inductive A :=
   | Cut
-  | Call : C -> A
-  | App : A -> Tm -> A.
+  (* | Call : C -> A *)
+  | App : C -> list Tm -> A.
   (* | PiImpl : V -> R_ A -> A -> A. *)
 Notation R := (@R_ A).
 
@@ -32,12 +36,10 @@ Axiom matching : Tm -> Tm -> Sigma -> option Sigma.
 
 Definition index := list R.
 Definition mode_ctx := P -> list mode.
-Record program := { (*depth : nat;*) rules : index; modes : mode_ctx }.
+Definition sigT := nat -> S.
+Record program := { (*depth : nat;*) rules : index; modes : mode_ctx; sig : sigT }.
 
-Inductive goal_ alt := Goal of program & A & list alt.
-Arguments Goal {_} _ _ _.
-Inductive alt := Alt of Sigma & list (goal_ alt).
-Notation goal := (goal_ alt).
+(* Inductive goal := Goal of program & Sigma & A. *)
 
 Axiom H : list mode -> list Tm -> list Tm -> Sigma -> option Sigma.
 Fixpoint select argsI (modes:list mode) (rules: list R) sigma :=
@@ -50,336 +52,866 @@ Fixpoint select argsI (modes:list mode) (rules: list R) sigma :=
     end
   end.
 
-Definition build_alt (pr: program) (gl:list goal) (alts:list alt) (s:Sigma) (r : R) : alt := 
-  Alt s ([seq Goal pr x alts | x <- r.(premises)] ++ gl).  
-
-Definition F pr pname args (gl:list goal) s (alts:list alt) :=
+Definition F pr pname args s :=
   let rules := pr.(rules) in
   let modes := pr.(modes) pname in
   let rules := select args modes rules s in
-  [seq match r with (s,r) => build_alt pr gl alts s r end | r <- rules].
+  rules.
 
-(* Axiom F : program -> P -> list Tm -> list goal -> Sigma -> list alt -> list alt. *)
+Inductive state :=
+  | KO : state
+  | OK : state
+  | Goal : program  -> A -> state
+  | Or  : state -> Sigma -> state -> state
+  | And : state -> state -> state
+  | CutOut : state
+  .
 
-Definition stack := list Tm.
+(* Notation "A ∧ B" := (And A B) (at level 13000).
+Notation "A ∨ B" := (Or A B) (at level 13000). *)
 
-Inductive run : stack -> alt -> list alt -> option (list alt * Sigma) -> Prop :=
-  (* | run_cut P s gl cta r _a :
+Inductive expand_res :=
+  | Expanded of state
+  | CutBrothers of state
+  | Failure
+  | Solved of Sigma.
 
-      run [::] (Alt s gl) cta r
-      (*--------------------------------------*) ->
-      run [::] (Alt s (Goal P Cut cta :: gl)) _a r *)
+Definition mkAnd left r :=
+  match r with
+  | Failure => Failure
+  | Expanded st => Expanded (And left st)
+  | CutBrothers st => CutBrothers (And left st)
+  | Solved s => Solved s
+  end.
 
-  | run_top s a :
+Definition mkOr left sr r :=
+  match r with
+  | Failure => Failure
+  | Expanded st => Expanded (Or left sr st)
+  | CutBrothers st => Expanded (Or left sr st) (* for now this is the rightmost brother *)
+  | Solved s => Solved s
+  end.
 
-      (*------------------------------------*)
-      run [::] (Alt s [::]) a (Some (a, s))
+Fixpoint cut st :=
+  match st with
+  | Goal _ _ => CutOut
+  | And x y => And (cut x) (cut y)
+  | Or x s y => Or (cut x) s (cut y)
+  | OK => CutOut
+  | KO => KO
+  | CutOut => CutOut
+  end.
 
-  | run_call s P pname args gl al a' al' r _a :
 
-      F P pname args gl s al = a' :: al' ->
-      run [::] a' (al'++al) r
-      (*------------------------------------*) ->
-      run args (Alt s (Goal P (Call (p pname)) _a :: gl)) al r
+Lemma cut_cut_same {a}: cut (cut a) = cut a.
+Proof. 
+  elim: a => //=.
+  + by move=> ? H => //= s A H1; rewrite H H1.
+  + by move=> ? H ? H1; rewrite H H1.
+Qed.
 
-  | run_back s P pname args gl a al r _a :
+Fixpoint big_and pr (a : list A) : state :=
+  match a with
+  | [::] => OK
+  | x :: xs => And (Goal pr x) (big_and pr xs)
+  end.
 
-      F P pname args gl s (a :: al) = [::] ->
-      run [::] a al r
-      (*----------------------------------------*) ->
-      run args (Alt s (Goal P (Call (p pname)) _a :: gl)) (a :: al) r
+Fixpoint big_or pr (s : seq (Sigma * R)) : state :=
+  match s with 
+  | [::] => KO
+  | [:: (_,r)] => big_and pr r.(premises)
+  | (_,r) :: ((s,_) :: _ as xs) => Or (big_and pr r.(premises)) s (big_or pr xs)
+  end.
 
-  | run_fail s P pname args gl _a :
-
-      F P pname args gl s [::] = [::] 
-      (**********************************) ->
-      run args (Alt s (Goal P (Call (p pname)) _a :: gl)) [::] None
- 
-  | run_sigma s P vname pname stack gl a al r :
-
-      s vname = Some (Code (p pname)) -> (* TODO: Comb -> App *)
-      run stack (Alt s (Goal P (Call (p pname)) a :: gl)) al r
-      (**********************************) ->
-      run stack (Alt s (Goal P (Call (v vname)) a :: gl)) al r
-
-  | run_app s P arg atom stack gl a al r :
-      run (rcons stack arg) (Alt s (Goal P atom a :: gl)) al r
-      (**********************************) ->
-      run stack (Alt s (Goal P (App atom arg) a :: gl)) al r
+Fixpoint expand s (st :state) : expand_res :=
+  match st with
+  | KO => Failure
+  | OK => Solved s
+  | CutOut => Failure
+  | Goal _ Cut  => CutBrothers OK
+  | Goal pr (App (v _) _) => Failure
+  | Goal pr (App (p pn) args) =>
+      let l := F pr pn args s in
+      if l is [:: (s1,_) & _] then Expanded (big_or pr l)
+      else Expanded KO
+  | Or st1 sr st2 =>
+      match expand s st1 with
+      | Solved s => Solved s
+      | Expanded st1 => Expanded (Or st1 sr st2)
+      | CutBrothers st1 => Expanded (Or st1 sr (cut st2))
+      | Failure => mkOr st1 sr (expand sr st2)
+      end
+  | And st1 st2 =>
+      match expand s st1 with
+      | Solved s1 => mkAnd st1 (expand s1 st2)
+      | Expanded st1 => Expanded (And st1 st2)
+      | CutBrothers st1 => CutBrothers (And st1 st2)
+      | Failure => Failure
+      end
+  end
 .
 
-Axiom suffix : seq alt -> seq alt -> Prop.
-Axiom suffix0 : forall a, suffix a [::].
-Axiom valid : seq alt -> Prop.
-Axiom append_alt : seq alt -> seq alt -> seq alt.
-Axiom append_alt_ok : forall a a1, valid a -> valid a1 -> valid (append_alt a a1).
-Axiom valid_run : forall a al a' s, valid (a :: al) -> run [::] a al (Some(a',s)) -> valid a'.
+Inductive run_res := Done of Sigma | Failed.
 
-(* Inductive run1_outcome (s : Sigma) gl : goal -> list alt -> list alt -> Sigma -> Prop :=
-| IsCut s'' cta P a' s' a'' :
-    run [::] (Alt s'' gl) cta (Some(a',s')) ->
-    run1_outcome s gl (Goal P Cut cta) a'' a'  s'
-| Fails g a' s' a1 a2 :
-    run [::] (Alt s [:: g]) [::] None ->
-    run [::] a1 a2 (Some(a',s')) ->
-      run1_outcome s gl g (a1::a2) a' s'
-| NotCut g P cta a a' a'' s' s'' :
-    ~ (g = Goal P Cut cta) ->
-    run [::] (Alt s [:: g]) [::] (Some(a,s'')) ->
-    run [::] (Alt s'' gl) (append_alt a a'') (Some(a',s')) ->
-      run1_outcome s gl g a'' a' s'.
+Inductive run : Sigma -> state -> run_res -> state -> Prop :=
+  | run_done {s st s'} :
+      expand s st = Solved s' ->
+      run s st (Done s') st
+  | run_fail {s st st1} :
+      expand s st = Failure ->
+      run s st Failed st1
+  | run_cut {s st st1 st2 r} :
+      expand s st = CutBrothers st1 ->
+      run s st1 r st2 ->
+      run s st r st2 
+  | run_step {s st st1 st2 r} :
+      expand s st = Expanded st1  ->
+      run s st1 r st2 ->
+      run s st r st2
+.
 
-
-Lemma run1P s g gl a' a'' s' :
-  valid ((Alt s (g :: gl)) :: a'') ->
-  run [::] (Alt s (g :: gl)) a'' (Some(a',s')) ->
-  run1_outcome s gl g a'' a' s'.
-Proof. *)
-(* case: g => p atom cta.
-elim: atom.
-  move=> H H1; apply: IsCut. inversion H1; subst. by eassumption.
-  move=> [pn|vn] Hv H; inversion H; subst.
-  have [[Hf [x[ax[def_a Hx]]]]|[_a Ha]] : (run [::] a'0 al' None /\ exists x ax,x :: ax = a /\ run [::] x ax (Some (a', s'))) \/
-                                  (exists _a, run [::] a'0 al' (Some (_a, s'))).
-    admit.
-  admit.
-  admit.
-  admit.
-  admit.
-move=> atom IH arg Hv H; inversion H; subst.
-
-
-move=> Valid H. 
-remember (Alt _ _) as a eqn:Ha.
-remember (Some _) as r eqn:Hr.
-remember [::] as stk eqn:Hs.
-elim: H Ha Hr Hs.
-  move=> P s1 gl1 cta {}r _a Hr IH [? ? ? ? _]; subst; apply: IsCut; by eassumption.
-  by [].
-  move=> s1 P pn args gl1 a1 a2 a3 a4 {}r a5 Hf Hr IH [? ? ? ? ?]. subst.
-inversion H; subst => {H}.
-  apply: IsCut; by eassumption.
-- admit.
-- apply: Fails. apply: run_fail. admit. assumption.
-
-
- *)
-(* Admitted. *)
-
-Lemma run_cut_gl P cta s g gl a' a'' s' {stk}:
-  run stk (Alt s (g :: gl)) a'' (Some(a',s')) ->
-  g = Goal P Cut cta ->
-  exists s'', run stk (Alt s'' gl) cta (Some(a',s')).
-Proof. move=> H1 ?; subst; inversion H1; eexists; eassumption. Qed.
-
-Lemma run_call_pn_empty P cta pn s g gl a' a'' s' stk :
-  run stk (Alt s (g :: gl)) a'' (Some(a',s')) ->
-  g = Goal P (Call (p pn)) cta ->
-  F P pn stk gl s a'' = [::] ->
-  exists x xs, x :: xs = a'' /\ run [::] x xs (Some(a',s')).
+Lemma run_Solved_id:
+  forall {s s1 s2 st1 st2},
+    expand s st1 = Solved s1 -> run s st1 (Done s2) st2 -> s2 = s1 /\ st1 = st2.
 Proof.
-  move=> H; inversion H; subst => {}H FP.
-    (* by []. *)
-    by injection H => ???; subst; rewrite H6 in FP.
-    injection H => ???; subst; exists a, al; auto.
-    by [].
-    by [].
+  move=> s s1 s2 st1 st2 + H.
+  remember (Done s2) as D eqn:HD.
+  case: H HD => //=; clear.
+  by move=> s st1 s3 H1 [] ?; rewrite H1=> -[] ?; subst.
+  by move=> s st st1 st2 r H H1 ?; rewrite H.
+  by move=> s st st1 st2 ? H ; rewrite H.
 Qed.
 
-Lemma run_call_pn_some P cta pn s g gl a a' s' stk x xs:
-  run stk (Alt s (g :: gl)) a (Some(a',s')) ->
-  g = Goal P (Call (p pn)) cta ->
-  F P pn stk gl s a ++ a = x :: xs ->
-  run [::] x xs (Some(a',s')).
+Lemma run_Failure_and_Done {s A sol A'}:
+  expand s A = Failure -> run s A (Done sol) A' -> False.
+Proof. by inversion 2; subst; congruence. Qed.
+
+Lemma run_Solved_and_Failed {s A sol A'}:
+  expand s A = Solved sol -> run s A Failed A' -> False.
+Proof. inversion 2; subst; congruence. Qed.
+
+Lemma run_consistent: forall {a b c1 c2 r1 r2},
+  run a b c1 r1 -> run a b c2 r2 -> c1 = c2 /\ (c1 <> Failed -> r1 = r2).
 Proof.
-  move=> H; inversion H; subst => {}H FP; try by []; injection H => ???; subst;
-    by rewrite H6 in FP; inversion FP; subst.
+  move=> a b c1 + r1  + H.
+  elim:H; clear.
+  + move=> s st s' H r1 r2 H1. {
+    inversion H1; subst; clear H1 => //=; rewrite H in H0.
+      by move: H0 => -[] <-.
+      all: by []. }
+  + move=> s st st1 H r1 r2 H0.
+    inversion H0; subst; clear H0 => //=; by rewrite H in H1.
+  + move=> s st st1 st2 r H H1 IH r1 r2 H2.
+    inversion H2; subst => //; rewrite H in H0; try by [].
+    by move: H0 => -[] ?; subst; auto.
+  + move=> s st st1 st2 r H H1 IH r1 r2 H2.
+    inversion H2; subst; clear H2; rewrite H in H0; try by [].
+    by move: H0 => [] ?; subst; auto.
 Qed.
 
-Lemma run_var_gl P cta vname s g gl a' a'' s' stk :
-  run stk (Alt s (g :: gl)) a'' (Some(a',s')) ->
-  g = Goal P (Call (v vname)) cta ->
-  exists x xs, 
-    (x :: xs = a'' \/ (exists pn, s vname = Some (Code (p pn)) /\ F P pn stk gl s a'' ++ a'' = x :: xs)) 
-      /\ run [::] x xs (Some(a',s')).
-Proof. 
-  move=> H1 ?; subst; inversion H1; subst.
-  inversion H10; subst; do 2 eexists; split; auto.
-  right; eexists; split; try eassumption.
-    rewrite H11; reflexivity.
-    auto.
+Lemma run_cut_simpl pr s3 s4 s2:
+  run s3 (Goal pr Cut) (Done s2) s4 -> expand s3 OK = Solved s2 /\ s4 = OK.
+Proof.
+  inversion 1; subst => //=.
+  move: H1 => //= [] ?; subst.
+  inversion H2; subst => //.
 Qed.
 
-Lemma run_inconsistent:
-  forall {stk g a s1 s2}, run stk g a s1 -> run stk g a s2 -> s1 = s2.
+Lemma run_solved_same_subst {A s1 s2 s3 B}:
+   expand s1 A = Solved s2 ->
+    run s1 A (Done s3) B ->
+      s2 = s3.
 Proof.
-  move=> stk g a s1 + H.
-  elim: H.
-    (* move=> ??????? IH ? H1; inversion H1; subst. by specialize (IH _ H7). *)
-    by move=> ??? H; inversion H.
-    move=> ?????????? HF H IH ? H1. 
-      inversion H1; subst; rewrite HF in H9; try by [].
-        injection H9; move=> ??; subst; auto.
-    by move=> ????????? HF ? IH ? H1; inversion H1; subst; auto; rewrite HF in H9.
-    move=> ?????? HF ? H; inversion H; subst; auto.
-      by rewrite H8 in HF.
-    move=> ????????? H H1 ?? H2.
-      inversion H2; subst.
-      rewrite H10 in H; inversion H; subst; auto.
-    move=> ????????? H ?? H1; inversion H1; auto.
+  remember (Done _) as D eqn:HD.
+  move=> + H.
+  elim: H s2 s3 HD; clear.
+  + by move=> s1 A s2 H s3 ? [] <-; rewrite H => -[].
+  + by congruence.
+  + by congruence.
+  + by congruence.
 Qed.
 
-Lemma FProp {P pn args gl1 gl2 s al1 al2 r}: 
-  F P pn args gl1 s al1 = [::] ->
-    F P pn args gl2 s al2 = r ->
-      r = [::].
+Lemma run_and_complete {s g1 g2 s' st} :
+  run s (And g1 g2) (Done s') st ->
+    (exists il ir s'', st = And il ir /\ run s g1 (Done s'') il /\ run s'' g2 (Done s') ir).
 Proof.
-  unfold F.
-  destruct select => //=.
+  remember (And _ _) as g0 eqn:Hg0.
+  remember (Done _) as s1 eqn:Hs1.
+  move => H.
+  move: g1 g2 Hg0 s' Hs1.
+  elim: H => {st s s1 g0} /= [s st s'|s st|s st st1 st2 r|] => //=.
+  - move=> + st_l st_r ? r [?]; subst => //=.
+    case L: expand => [|||x] //; case R: expand => //= -[?]; subst.
+    by exists st_l, st_r, x; repeat split; constructor.
+  - move=> + Hr + st_l st_r ? s'' ?; subst => //=.
+    case L: expand => [|st0||s'] // => [[?]|]; subst.
+    - move=> /(_ _ _ erefl _ erefl) [il [ir [s']]] [-> [ IHl IHr]].
+      exists il, ir, s'; split=> //; split.
+      by apply: run_cut L IHl.
+      by apply: IHr.
+    - case R: expand => //= -[?]; subst.
+      move=> /(_ _ _ erefl _ erefl) [il [ir [s''']]] [-> [ IHl IHr]].
+      exists il, ir, s'''; split=> //; split.
+      - by apply: IHl.
+      - move: (run_solved_same_subst L IHl) => ?; subst.
+        apply: run_cut R IHr.
+  - move=> s ? A' C ? + H1 + A B ? s' ?; subst => //=.
+    case E1: expand => //= [|s1].
+    - move=> [?]; subst.
+      move => /(_ _ _ erefl _ erefl) [il [ir [s''']]] [-> [ IHl IHr]].
+      exists il, ir, s'''; repeat split => //=.
+      by apply: run_step E1 IHl.
+    - case E2: expand => //= [st] [] ?; subst.
+      move=> /(_ _ _ erefl _ erefl) [il [ir [s''']]] [? [ IHl IHr]]; subst.
+      move: (run_Solved_id E1 IHl) => [] ??; subst.
+      exists il, ir, s1; repeat split => //=.
+      apply: run_step E2 IHr.
 Qed.
 
-Lemma FSuff {P pn args g1 g2 s al1 x xs y ys}: 
-  let f := fun x => match x with Alt s g => Alt s (g ++ g2) end in
-  F P pn args g1 s al1 = x :: xs ->
-    F P pn args (g1 ++ g2) s al1 = y :: ys ->
-      y :: ys = [seq f a | a <- x :: xs].
+Lemma run_and_correct {s0 s1 s2 g1 g2 il ir} :
+    run s0 g1 (Done s1) il -> run s1 g2 (Done s2) ir ->
+      run s0 (And g1 g2) (Done s2) (And il ir).
 Proof.
-  unfold F; destruct select => //=.
-  destruct p0.
-  move=> [] ?? [] ??; subst.
-  unfold build_alt.
-  f_equal.
-  by rewrite catA.
-  induction l; auto; simpl.
-  f_equal; auto.
-  destruct a.
-  by rewrite catA.
+  remember (Done _) as ds1 eqn:Hds1.
+  move => H.
+  move: s1 s2 g2 ir Hds1.
+  elim: H => //=; clear.
+  + move=> + + s' + s1 s2 g2 ir [] ? H1; subst.
+    remember (Done s2).
+    move: s2 Heqr.
+    elim: H1 => //=; clear.
+    + move=> s st s' H s2 [] ? s0 g1 H1; subst.
+      apply: run_done => //=; rewrite H1 H => //=.
+    + move=> s g2 st1 st2 r H H1 IH s2 ? s0 g1 H2; subst.
+      apply: run_cut => //=.
+      + rewrite H2 H => //=.
+      + apply: IH => //=.
+    + move=> s g2 st1 st2 r H H1 IH s2 ? s0 g1 H2; subst.
+      apply: run_step => //=.
+      + by rewrite H2 H.
+      + by apply: IH _ H2.
+  + move=> s0 g1 st1 il r H H1 IH s3 s2 g2 ir ? H2; subst.
+    apply: run_cut => //=.
+    + by rewrite H.
+    + by apply: IH _ H2.
+  + move=> s0 g1 st1 il ? H H1 IH s1 s2 g2 ir ? H2; subst.
+    apply: run_step => //=.
+    + by rewrite H.
+    + by apply: IH erefl H2.
 Qed.
+ 
 
-
-
-Corollary FSuff_singleton {P pn args gl s al1 x xs y ys}: 
-  let f := fun x => match x with Alt s g => Alt s (g ++ gl) end in
-  F P pn args [::] s al1 = x :: xs ->
-    F P pn args gl s al1 = y :: ys ->
-      y :: ys = [seq f a | a <- x :: xs].
-Proof. intros; apply (FSuff H0 H1). Qed.
-
-Definition alt_prefix g2 al' :=
-  [seq match a with | Alt s g => Alt s (g ++ g2) end | a <- al'].
-
-
-
-Lemma run_pref_none s g1 g2 a a2 stk r:
-  run stk (Alt s g1) (a ++ a2) None ->
-  run stk (Alt s (g1 ++ g2)) a r ->
-  r = None.
+Lemma run_and_fail {s g1 g2 st}:
+  run s (And g1 g2) Failed st ->
+    run s g1 Failed st \/ (exists s' st', run s g1 (Done s') st' /\ run s' g2 Failed st).
 Proof.
-  remember None as o eqn:Ro.
-  remember (Alt _ _) as A eqn:RA.
-  remember (cat _ _) as C eqn:HC.
   move=> H.
-  move: s g1 g2 r a2 HC RA Ro.
-  elim: H.
-    (* move=> ?????? H IH ?? [] ????? H1; subst.
-      eapply IH; try reflexivity.
-      inversion H1; subst; eassumption. *)
-    by [].
-    (* caso run_call *)
-    move=> ?????? a'' ? OO ? HF H IH ?????? H0 ? H1; subst.
-      inversion H0; subst; clear H0.
-      { inversion H1; clear H1; subst.
-        (* epose proof (FSuff HF H9). *)
-        admit.
-        2:auto.
-        by epose proof (FProp H9 HF) as HS.
-      }
-    move=> ????????? H H1 IH ? ???? HC [] ??? H2; subst.
-      { inversion H2 => //; subst; clear H2.
-        by pose proof (FProp H H10).
-        inversion HC; subst.
+  remember (And _ _) as A eqn:HA.
+  remember Failed as F eqn:HF.
+  move: g1 g2 HA HF.
+  elim: H => //=; clear.
+  + move=> s st st1 + g1 g2 ? ?; subst => //=.
+    case E: expand => [|||s2] //=.
+    + by move=> _; left; apply: run_fail.
+    + case F: expand => //=.
+      move=> _; right.
+      exists s2, g1; split.
+        - by apply run_done.
+        - by apply run_fail.
+  + move=> s ? st1 st2 ? + H IH g1 g2 ? ?; subst => //=.
+    case E: expand => //=.
+    - move=> [] ?; subst.
+      move: (IH _ _ erefl erefl) => [].
+      + by left; apply: run_cut E _.
+      + move=> [? [? []]] H1 H2.
+        by right; do 2 eexists; split; [|eassumption]; apply: run_cut E H1.
+    - case F: expand => //= -[] ?; subst.
+      move: (IH _ _ erefl erefl) => []; [by auto|].
+      move=> [? [? []]] H1 H2.
+      epose proof (run_Solved_id E H1) as []; subst.
+      by right; do 2 eexists; split; [eassumption|apply: run_cut F H2].
+  + move=> s ? st1 st2 ? + H1 IH g1 g2 ??; subst => //=.
+    case E: expand => //=.
+    + move=> [] ?; subst.
+      move: (IH _ _ erefl erefl) => [] {IH}.
+      + by left; apply: run_step E _.
+      + move=> [? [? []]] H2 H3.
+        by right; do 2 eexists; split; [apply: run_step E H2|].
+    + case F: expand => //= -[] ?; subst.
+      move: (IH _ _ erefl erefl) => [] {IH}; [by auto|].
+      move=> [? [? []]] H2 H3.
+      epose proof (run_Solved_id E H2) as []; subst.
+      right; do 2 eexists; split; [by eassumption|].
+      by apply: run_step F H3.
+Qed.
 
-        (* IH is useless... *)
-        admit.
-      }
-    move=> ?????? HF ?????? [] ??? H; subst. inversion H; subst => //.
-      by pose proof (FProp HF H8).
-    move=> ????????? H H1 IH ?????? [] ??? H2; subst.
-      inversion H2; subst.
-      rewrite H in H10.
-      move: H10 => [] ?; subst.
-      eapply IH; try reflexivity.
-      eassumption.
-    move=> ????????? H IH ?????? [] ??? H1; subst; inversion H1; subst.
-    eapply IH; try reflexivity.
-    eassumption.
+Inductive expand_no_cut_failure : Sigma -> state -> state -> Prop :=
+  | expand_no_cut_failure_fail {s st} :
+      expand s st = Failure ->
+      expand_no_cut_failure s st st
+  | expand_no_cut_failure_step {s st st1 st2} :
+      expand s st = Expanded st1  ->
+      expand_no_cut_failure s st1 st2 ->
+      expand_no_cut_failure s st st2
+.
+
+Inductive expand_no_cut : Sigma -> state -> Prop :=
+  | expand_no_cut_solved {s' s g} : expand s g = Solved s' -> expand_no_cut s g
+  | expand_no_cut_failure1 {s g}    : expand s g = Failure   -> expand_no_cut s g
+  | expand_no_cut_expanded {s g g'} : 
+    expand s g = Expanded g' -> expand_no_cut s g' -> expand_no_cut s g.
+
+Inductive expand_with_cut : Sigma -> state -> Prop :=
+  | expand_with_cut_cb {s g g'} : expand s g = CutBrothers g' -> expand_with_cut s g
+  | expand_with_cut_exp {s g g'} : expand s g = Expanded g' -> expand_with_cut s g' -> expand_with_cut s g.
+
+Inductive expand_will_fail: Sigma -> state -> Prop :=
+  | expand_will_fail_fail {s g}    : expand s g = Failure -> expand_will_fail s g
+  | expand_will_fail_cut {s g g'} : expand s g = CutBrothers g' -> expand_will_fail s g' -> expand_will_fail s g
+  | expand_will_fail_exp {s g g'} : expand s g = Expanded g' -> expand_will_fail s g' -> expand_will_fail s g
+.
+
+Lemma expand_no_cutP {s1 g1 g2 g3}:
+  expand s1 g1 = Expanded g2 -> 
+    expand_no_cut s1 g1 ->
+      run s1 g2 Failed g3 ->
+        expand_no_cut s1 g2.
+Proof.
+  move=> + H.
+  move: g2 g3.
+  elim: H => //=.
+  move=> s' s g H g2 g3 H1 H2.
+    inversion H2; subst; clear H2 => //=; rewrite H1 in H; try by [].
+  move=> s g H g2 g3 H1 H2.
+    remember Failed.
+    move: s1 g1 g H H1 Heqr => _ _.
+    elim: H2 => //=; clear.
+    by move=> s st _ H g H1 H2 _; apply: expand_no_cut_failure1 H.
+    by move=> s st st1 st2 r H H1 IH g H2 H3 H4; subst; rewrite H2 in H3.
+    by move=> s st st1 st2 r H H1 IH g H2 H3 H4; subst; rewrite H2 in H3.
+  by move=> s g g' H H1 IH g2 g3 + H3; rewrite H => -[] ?; subst.
+Qed.
+
+Lemma expand_cut_fail {s A SOL}:
+  expand s (cut A) = Solved SOL -> False.
+Proof.
+  elim: A s SOL => //=.
+  + move=> s IH s' A H s'' SOL //=.
+    case E: expand => //=.
+    + case F: expand => //= -[] ?; subst.
+      apply: H F.
+    + by move=> [] ?; subst; apply: IH E.
+  + move=> s IH1 A IH2 s' SOL.
+    case E: expand => //=.
+    case F: expand => //= -[] ?; subst.
+    apply: IH2 F.
+Qed.
+
+Lemma expand_cut_CB {s A B}:
+  expand s (cut A) = CutBrothers B -> False.
+Proof.
+  elim: A s B => //=.
+  + move=> AL IH s' AR H s B => //=.
+    case X: expand => //=.
+    case Y: expand => //=.
+  + move=> A IHA B IHB s C.
+    case X: expand => //=.
+    + move=> [] ?; subst; apply: IHA X.
+    + case: expand => //=? -[]?; subst.
+      apply: expand_cut_fail X.
+Qed.
+
+Lemma expand_cut_expanded {s A B}: expand s (cut A) = Expanded B -> False.
+Proof.
+  elim: A s B => //=; clear.
+    move=> s IH s' A H s'' B //=; case E: expand => //=.
+    + by move=> [] ?; subst; f_equal; apply: IH E.
+    + by move: (expand_cut_CB E).
+    + case F: expand => //=.
+      - move=> [] ?; subst.
+        by move: (H _ _ F) => ?; subst.
+      - by move: (expand_cut_CB F).
+  move=> s0 IH0 s1 IH1 s A; case E: expand => //=.
+    by move=> [] ?; subst; move: (IH0 _ _ E) => ?; subst.
+  case F: expand => //= -[] ?; subst.
+  by move: (IH1 _ _ F) => ?; subst.
+Qed.
+
+Axiom classic : forall P : Prop, P \/ ~ P.
+
+Lemma expand_cut_result {s A r}:
+  expand s (cut A) = r -> (exists B, r = Expanded B) \/ r = Failure.
+Proof.
+  elim: A s r => //=; auto.
+  + move=> A IH a A' HA' s r //=.
+    case H: expand => //=.
+    + by move=>?; subst; left; eexists.
+    + by move=>?; subst; left; eexists.
+    + case X: expand => //=?; subst; auto.
+      + by left; eexists.
+      + by left; eexists.
+      + apply: HA' X.
+    + apply IH in H as [[]|?] => //=.
+  + move=> s1 IH1 s2 IH2 s3 r.
+    case H: expand => ?; subst; auto.
+    + by left; eexists.
+    + apply IH1 in H as [[]|?] => //=.
+    + apply IH1 in H as [[]|?] => //=.
+Qed.
+
+Lemma expand_cut_result1 s A:
+  expand s (cut A) = Failure \/ exists x, expand s (cut A) = (Expanded x).
+Proof.
+  case X: (expand s (cut A)).
+  + by right; eexists.
+  + by move: (expand_cut_CB X).
+  + by left.
+  + by move: (expand_cut_fail X).
+Qed.
+
+Lemma run_cut_fail {s A SOL X} :
+  run s (cut A) (Done SOL) X -> False.
+Proof.
+  remember (cut A) as C eqn:HC.
+  remember (Done SOL) as D eqn:HD.
+  move=> H.
+  move: A SOL HC HD.
+  elim: H; clear => //=.
+  + by move=> ??? H ?? ? [] ?; subst; apply: expand_cut_fail H.
+  + move=> s st st1 st2 r H H1 IH A SOL ??; subst.
+    by move: (expand_cut_CB H).
+  + move=> s st st1 st2 r H H1 IH A SOL ??; subst.
+    by apply expand_cut_expanded in H.
+Qed.
+Inductive chooseB : Sigma -> state -> state -> state -> Prop :=
+  | chooseB_CB {s A cb B} : expand s A = CutBrothers cb -> chooseB s A B (cut B)
+  | chooseB_Fail {s A B} : expand s A = Failure -> chooseB s A B B
+  | chooseB_Done {s s' A B} : expand s A = Solved s' -> chooseB s A B B
+  | chooseB_Exp {s A A' B B'} : expand s A = Expanded A' -> chooseB s A' B B' -> chooseB s A B B'
+  .
+
+Lemma chooseBP {s A B C} :
+  chooseB s A (cut B) C -> cut B = C.
+Proof.
+  remember (cut _) as CC eqn:HCC.
+  move=> H; move: B HCC.
+  elim: H; clear => //=.
+  by intros; subst; rewrite cut_cut_same.
+Qed.
+
+Lemma chooseB_cut_result s A B:
+  chooseB s A B B \/ chooseB s A B (cut B).
+Proof.
+  
 Admitted.
 
-
-
-(* Lemma run_x_y s g gl a' a'' s' :
-  valid ((Alt s (g :: gl)) :: a'') ->
-  run [::] (Alt s (g :: gl)) a'' (Some(a',s')) ->
-  (exists P cta s'' a, g = Goal P Cut cta,
-                 run [::] (Alt s'' gl) cta (Some(a',s')))
-  \/
-  (exists s'' a, (froall P cta, ~ (g = Goal P Cut cta)) /\
-                 run [::] (Alt s [:: g]) [::] (Some(a,s'')) /\
-                 run [::] (Alt s'' gl) (append_alt a a'') (Some(a',s')))
-  \/
-  (run [::] (Alt s [:: g]) a'' None /\ exists a1 a2, a1 :: a2 = a'' /\ run [::] a1 a2 (Some(a',s'))).
+Lemma chooseB_cut_cut {s A B}:
+  chooseB s A (cut B) (cut B).
 Proof.
-Admitted. *)
+  move: (chooseB_cut_result s A (cut B)) => []; [by auto|].
+  by rewrite cut_cut_same; auto.
+Qed.
 
+Lemma chooseB_expanded {s1 A' A B B'}:
+  expand s1 A = Expanded A' -> chooseB s1 A B B' -> chooseB s1 A' B B'.
+Proof. by move=> + H; elim: H A'; clear; congruence. Qed.
 
-(* Lemma run_x_cut_y P s g1 g2 cta _a a' s' s'' :
-  run [::] (Alt s (g1 ++ [:: Goal P Cut cta] ++ g2)) [::] (Some(a',s')) ->
-  run [::] (Alt s g1) [::] (Some(_a,s'')) ->
-  run [::] (Alt s'' g2) cta (Some(a',s')).
+Inductive expand_all: Sigma -> state -> expand_res -> Prop :=
+  | expand_all_done {s st r} : expand s st = (Solved r) -> expand_all s st (Solved r)
+  | expand_all_fail {s st} : expand s st = Failure -> expand_all s st Failure
+  | expand_all_cut {s st st1 r} : expand s st = CutBrothers st1 -> expand_all s st1 r -> expand_all s st r
+  | expand_all_exp {s st st1 r} : expand s st = Expanded st1 -> expand_all s st1 r -> expand_all s st r.
+
+Lemma run_expand_all_solved {s0 s1 s2 A B}:
+  expand_all s0 A (Solved s2) -> run s0 A (Done s1) B -> s1 = s2.
 Proof.
-move: ([::] : list alt) cta (suffix0 cta).
-elim: g1 => [|g gl IH] e cta Hcta.
-  rewrite cat0s cat_cons cat0s => H.
-  inversion H; subst => {H} H1.
-  by inversion H1; subst => {H1}.
-rewrite cat_cons => H H1.
-case/run_x_y: H1 => s1 [a [H1 H2]]. *)
+  remember (Solved s2) as S eqn:HS => H.
+  elim: H s1 s2 B HS; clear => //=.
+  + by move=> s0 A r H s1 s2 B []<- H1; move: (run_solved_same_subst H H1).
+  + all:
+    move=> s0 A AC ? H1 H2 IH s1 s2 B ? H3; inversion H3; clear H3; try congruence; subst; 
+    move: H0; rewrite H1 => -[]?; subst; by apply: IH erefl H4.
+Qed.
 
+Lemma expand_no_cut_failure_split {s A B AB}: 
+  expand_no_cut_failure s (And A B) AB ->
+    (exists X, expand_no_cut_failure s A X) \/ (exists s' X, expand_all s A (Solved s') /\ expand_no_cut_failure s' B X).
+Proof.
+  remember (And A B) as And eqn:HAnd.
+  move=> H; elim: H A B HAnd; clear.
+  + move=> s ? + A B ?; subst => //=.
+    case X: expand => //=.
+    + by left; eexists A; apply: expand_no_cut_failure_fail.
+    + case Y: expand => //= _; right; do 2 eexists; split.
+      + apply: expand_all_done X.
+      + by apply: expand_no_cut_failure_fail.
+  + move=> s st st1 st2 + H1 + A B ?; subst => //=.
+    case X: expand => //=.
+    + move=> []?;subst.
+      move=> /(_ _ _ erefl) [] [].
+      + move=> X1 H; left; eexists; apply: expand_no_cut_failure_step X H.
+      + move=> X1 [X2 [H2 H3]]; right.
+        do 2 eexists; split.
+        + apply: expand_all_exp X H2.
+        + apply: H3.
+    + case Y: expand => //= [A'] [] ?; subst.
+      move=> /(_ _ _ erefl) [].
+      + by left.
+      + move=> [s' [B' [H2 H3]]]; right.
+        do 2 eexists; split; try eassumption.
+        inversion H2; subst; try congruence; clear H2.
+        move: H6; rewrite X => -[]?; subst.
+        by apply: expand_no_cut_failure_step Y H3.
+Qed.
 
-Definition is_det P p args :=
-  forall a s0 s, run args (Alt s0 [:: Goal P (Call p) [::]]) [::] (Some(a,s)) -> a = [::].
+Lemma run_or_correct {s1 s2 A B SOL A' B'}:
+  (chooseB s1 A B B' /\ run s1 A (Done SOL) A') \/ 
+  (expand_no_cut_failure s1 A A' /\ run s2 B (Done SOL) B') ->
+  run s1 (Or A s2 B) (Done SOL) (Or A' s2 B').
+Proof.
+  move=> [] [].
+  - remember (Done SOL) as DS eqn:HS.
+    move=> + H; move: s2 B SOL B' HS.
+    elim: H => //=; clear.
+    - move=> s1 A SOL + s2 B SOL' B' [] ? H; subst; move: s2 SOL'.
+      elim: H; clear; try congruence.
+      move=> s1 s' A B H; rewrite H => s2 SOL' [] <-.
+      by apply: run_done => //=; rewrite H.
+    - move=> s1 A AC A' r H H1 + s2 B SOL B' ? H2; subst.
+      move=> /(_ _ _ _ _ erefl) IH.
+      inversion H2; subst; try congruence; clear cb H0.
+      apply: run_step => //=.
+      + by rewrite H.
+      + apply: IH chooseB_cut_cut.
+    - move=> s1 A st1 st2 r H H1 + s2 B SOL B' ? H2; subst.
+      move=> /(_ _ _ _ _ erefl) IH.
+      apply: run_step => //=.
+      + by rewrite H.
+      + apply: IH (chooseB_expanded H H2).
+  - move=> H.
+    elim: H s2 B B' SOL; clear.
+    + move=> + + + s2 B B' SOL H1.
+      remember (Done SOL) as DS eqn:HDS.
+      elim: H1 SOL HDS => //=; clear.
+      + by move=> s2 B SOL H SOL' [] ? s1 A H1; apply: run_done =>//=; rewrite H1 H.
+      + move=> s2 B BC B' r H H1 + SOL ? s1 A H2; subst.
+        move=> /(_ _ erefl _ _ H2) IH.
+        apply: run_step _ IH => //=.
+        by rewrite H2 H.
+      + move=> s2 B BE B' r H H1 + SOL ? s1 A H2; subst.
+        move=> /(_ _ erefl _ _ H2) IH.
+        apply: run_step _ IH => //=.
+        by rewrite H2 H.
+    + move=> s1 A EA A' H H1 + s2 B B' SOL H2.
+      move=> /(_ _ _ _ _ H2) IH.
+      apply: run_step _ IH => //=.
+      by rewrite H.
+Qed. 
 
-Definition Gamma := C -> S.
+Lemma run_or_complete {s1 s2 A B SOL E}:
+  run s1 (Or A s2 B) (Done SOL) E ->
+    (exists A' B', chooseB s1 A B B' /\ E = Or A' s2 B' /\ run s1 A (Done SOL) A') \/ 
+      exists A' B', expand_no_cut_failure s1 A A' /\ E = (Or A' s2 B') /\ run s2 B (Done SOL) B'.
+Proof.
+  move=> H.
+  remember (Or _ _ _) as O eqn:HO.
+  remember (Done _) as D eqn:HD.
+  move: s2 A B SOL HO HD.
+  elim: H; clear => //=.
+  + move=> s st s' + s2 A B SOL ? [] ?; subst => //=.
+    case E: expand => //=.
+      case F: expand => //= -[] ?; subst.
+      by right; exists A, B; repeat split; auto; [apply: expand_no_cut_failure_fail E| apply: run_done].
+    move=> [] ?; subst; left.
+    exists A; eexists.
+    split.
+    apply: chooseB_Done E.
+    by split; auto; apply run_done.
+  + move=> s ? st1 st2 ? + H1 IH s2 A B SOL ? ?; subst => /=.
+    case E: expand => //=.
+    by case F: expand => //=.
+  + move=> s ? st1 st2 ? + H1 IH s2 A B SOL ?? ; subst => //=.
+    case E: expand => [s4|||s4] //=.
+    + move=> [] ?; subst.
+      move: (IH _ _ _ _ erefl erefl) => [H|[A' [B' [H [? H0]]]]] {IH}; subst.
+      - move: H => [A' [B' [H [H0 H2]]]]; subst.
+        left; do 2 eexists.
+        split.
+        apply: chooseB_Exp E H.
+        split; [reflexivity | apply: run_step E H2 ].
+      - by right; exists A', B'; repeat split; auto; apply: expand_no_cut_failure_step E H.
+    + move=> [] ?; subst.
+      move: (IH _ _ _ _ erefl erefl) => [H|[A' [B' [H [? H0]]]]] {IH}; subst.
+      - move: H => [A' [B' [H [H0 H2]]]]; subst.
+        left; do 2 eexists.
+        apply chooseBP in H; split; subst.
+        apply: chooseB_CB E.
+        split; [reflexivity|apply: run_cut E H2].
+      - by right; exists A', B'; split; auto; move: (run_cut_fail H0).
+    + case F: expand => [ss|ss||] //=.
+      - move=> [] ?; subst.
+        move: (IH _ _ _ _ erefl erefl) => [H|[A' [B' [H [? H0]]]]] {IH}; subst.
+        move: H => [A' [B' [H [H0 H2]]]]; subst.
+        by destruct (run_Failure_and_Done E H2).
+        right; exists A', B'; repeat split; auto; apply: run_step F H0.
+      - move=> [] ?; subst.
+        move: (IH _ _ _ _ erefl erefl) => [H|[A' [B' [H [? H0]]]]] {IH}; subst.
+        move: H => [A' [B' [H [H0 H2]]]]; subst.
+        by destruct (run_Failure_and_Done E H2).
+        by right; exists A', B'; repeat split; auto; apply: run_cut F H0.
+Qed.
 
-Axiom lookup_Gamma : Gamma -> C -> list Tm -> B * list (S * Tm) * list (S * Tm). 
+Lemma run_expand_no_cut_failure {s A ign} : 
+  expand_no_cut_failure s A ign -> 
+    run s A Failed ign.
+Proof.
+  move=> H; elim: H => [{}s {}st| {}s {}st st1 st2] H.
+  + by apply: run_fail H.
+  + by move=> _ H2; apply: run_step H H2.
+Qed.
 
-Fixpoint allp2 {A B} (f : A -> B -> Prop)  l :=
-  match l with
-  | [::] => True
-  | [:: (x,y) & l] => f x y /\ allp2 f l
+Lemma expand_no_cut_failure_expanded {s1 s2 g1 g2}:
+   expand s1 g1 = Expanded s2 ->
+    expand_no_cut_failure s1 g1 g2 ->
+      expand_no_cut_failure s1 s2 g2.
+Proof.
+  move=> + H; elim: H s2; [congruence|]; clear.
+  move=> s1 st st1 g2 H; rewrite H => H1 IH g1 []?; subst.
+  inversion H1; clear H1; subst.
+  - by apply: expand_no_cut_failure_fail.
+  - by apply: expand_no_cut_failure_step (H0) _; apply IH.
+Qed.
+
+Lemma run_or_fail {s1 s2 g1 g2 st}:
+  run s1 (Or g1 s2 g2) Failed st ->
+    run s1 g1 Failed st /\ (expand_no_cut s1 g1 -> run s2 g2 Failed st).
+Proof.
+  move=> H.
+  remember (Or _ _ _) as O eqn:HO.
+  remember Failed as F eqn:HF.
+  move: s2 g1 g2 HO HF.
+  elim: H; clear => //=.
+  + move=> s st s' + s2 g1 g2 HO _; subst => /=.
+    case E: expand => //=.
+    case F: expand => //=.
+    by move=> _; split; intros; apply run_fail.
+  + move=> s ? st1 st2 ? + H1 IH s2 g1 g2 ? ?; subst => /=.
+    case E: expand => //=.
+    by case F: expand => //=.
+  + move=> s ? st1 st2 ? + H1 IH s2 g1 g2 ?? ; subst => //=.
+    case E: expand => [s4|||s4] //=.
+    + move=> [] ?; subst.
+      move: (IH _ _ _ erefl erefl) => [] HL HR {IH}.
+      split; [by apply: run_step E _|] => H.
+      inversion H1; subst; clear H1; move: H0 => //=.
+      + case F: expand => //=; case: expand => //= _.
+        apply: HR (expand_no_cut_failure1 F).
+      + by case F: expand => //=; case G: expand => //=.
+      + by epose proof (expand_no_cutP E H HL); auto.
+    + move=> [] ?; subst.
+      move: (IH _ _ _ erefl erefl) => [] HL HR.
+      split; [by apply: run_cut E HL|] => H.
+      inversion H; clear H; subst; rewrite E in H0 => //=.
+    + case F: expand => //= -[] ?; subst.
+      - move: (IH _ _ _ erefl erefl) => [] HL HR; split; [by []|] => HH.
+        by apply: run_step F (HR HH).
+      - move: (IH _ _ _ erefl erefl) => [] HL HR; split; [by []|] => HH.
+        by apply: run_cut F (HR HH).
+Qed.
+
+Lemma expand_no_cut_cut {s A B}:
+  expand_no_cut s A -> expand s A = CutBrothers B -> False.
+Proof. by move=> H; elim: H B; congruence. Qed.
+
+Lemma run_Failed_cut {s s2 A B X Y}:
+   run s A Failed X ->
+    run s (Or A s2 (cut B)) Failed Y.
+Proof.
+  remember Failed as F eqn:HF.
+  move=> H.
+  elim: H s2 B Y HF; clear => //=.
+  + move=> s A _ H s2 B Y _.
+    move: (expand_cut_result1 s2 B) => [ | [D]] H1.
+    + by apply: run_fail => //=; rewrite H H1.
+    + by move: (expand_cut_expanded H1).
+  + move=> s A st1 st2 r H H1 IH s2 B Y ?; subst.
+    apply: run_step => //=.
+    + by rewrite H.
+    + apply: IH erefl.
+  + move=> s A st1 st2 r H H1 IH s2 B Y ?; subst.
+    apply: run_step => //=.
+    + by rewrite H.
+    + apply: IH erefl.
+Qed.
+
+Lemma run_or_fail1 {s1 s2 g1 g2 st aa}:
+    run s1 g1 Failed aa -> (expand_no_cut s1 g1 -> run s2 g2 Failed st) ->
+      run s1 (Or g1 s2 g2) Failed st.
+Proof.
+  move: (classic (expand_no_cut s1 g1)) => [].
+  + move=> H + /(_ H) => H1; move: H.  
+    remember Failed as F eqn:HF.
+    elim: H1 s2 g2 st HF; clear => //=.
+    + move=> s A _ H s2 B C _ H1 H2; subst.
+      remember Failed as F eqn:HF.
+      elim: H2 s A H H1 HF; clear => //=.
+      + by intros; apply run_fail => //=; rewrite H0 H1.
+      + intros; subst. 
+        apply: run_step => //=.
+        rewrite H3 H0 => //=.
+        by apply H2 => //=.
+      + intros.
+        apply: run_step => //=.
+        rewrite H3 H0 => //=.
+        by auto.
+    + intros; subst.
+      by move: (expand_no_cut_cut H3 H0).
+    + intros; subst.
+      apply: run_step=> //=.
+      + by rewrite H0 => //=.
+      + by apply: H2 => //=; apply: expand_no_cutP H0 H3 H1.
+  + remember Failed as F eqn:HF.
+    remember (Or _ _) as O eqn:HO.
+    move=> H1 H _.
+    elim: H H1 s2 g2 st HF O HO; clear => //=.
+    + by move=> s st st1 H []; apply expand_no_cut_failure1.
+    + move=> s st st1 st2 r H H1 IH H2 s2 g2 st0 ? O HO; subst.
+      apply: run_step => //=.
+      + rewrite H => //=.
+      + apply: run_Failed_cut H1.
+    + intros; subst.
+      apply: run_step => //=.
+      by rewrite H0.
+      apply: H2; auto.
+      move=> H4.
+      apply H3.
+      apply: expand_no_cut_expanded H0 H4.
+Qed.
+
+Lemma done_fail {s}: Done s <> Failed. by []. Qed.
+
+Lemma chooseB_complete s A B: exists X, chooseB s A B X.
+Proof.
+  (* move: (classic (expand_no_cut s A)) => [] H; [exists B|exists (cut B)].
+  + elim: H B; clear.
+    + move=> ??? H ?; apply: chooseB_Done H.
+    + move=> ?? H ?; apply: chooseB_Fail H.
+    + move=> ??? H _ IH ?; apply: chooseB_Exp H _; apply: IH. *)
+Admitted. 
+
+Module check.
+  Definition Gamma := V -> S.
+
+  Fixpoint eat r1 r2 :=
+    match r1, r2 with
+    | arr _ _ r1, arr _ _ r2 => eat r1 r2
+    | arr _ _ r1, _ => r1
+    | _, _ => r1
+    end.
+
+  Fixpoint incl d1 d2 :=
+    match d1, d2 with
+    | b Exp, b Exp => true
+    | b (d Func), b (d Func) => true
+    | b (d Func), b (d Pred) => true
+    | arr i l1 r1, arr i l2 r2 => incl l1 l2 && incl r1 r2
+    | arr i l1 _, x => incl l1 x
+    | arr o l1 r1, arr o l2 r2 => incl r1 r2
+    | _, _ => false
   end.
 
-#[bypass_check(guard)]
-Fixpoint sem P G ty (t : Tm) {struct t} :=
-  match ty, t with
-  | Base Exp, Data _ _ => True
-  | Base (Det d'), Code c args =>
-      let: (d,i, o) := lookup_Gamma G c args in
-      d = Det d' /\
-      if d is Det Func then allp2 (sem P G) i -> is_det P c args /\ True
-      else True
-  | Arr _ _ _, Lam _ _ _ _ => False
-  | _, _ => False
+  Fixpoint min m1 m2 :=
+    match m1, m2 with
+    | b Exp, b Exp => b Exp
+    | b (d Func), _ => m1
+    | b (d Pred), _ => m2
+    | arr i l1 r1, arr i l2 r2 => arr i (max l1 l2) (min r1 r2)
+    | arr o l1 r1, arr o l2 r2 => arr o (min l1 l2) (min r1 r2)
+    | _, _ => m1
+  end
+  with max m1 m2 := match m1, m2 with
+    | b Exp, b Exp => b Exp
+    | b (d Func), _ => m1
+    | b (d Pred), _ => m2
+    | arr i l1 r1, arr i l2 r2 => arr i (min l1 l2) (max r1 r2)
+    | arr o l1 r1, arr o l2 r2 => arr o (max l1 l2) (max r1 r2)
+    | _, _ => m1
   end.
 
-Definition checked P G :=
-  forall c args,
-  let: (f,i, o) := lookup_Gamma G c args in
-  sem P G (Base f) (Code c args).
+  Fixpoint infer (G: Gamma) tm :=
+    match tm with
+    | Code (v V) => (G V, true)
+    | Code (p P) => (G P, true)
+    | Data _ => (b Exp, true)
+    | Comb t1 t2 => 
+      match infer G t1 with
+      | (r, false) => (r, false)
+      | (r, _) => 
+        match infer G t2 with
+        | (r, false) => (r, false)
+        | (d1, true) => (eat r d1, incl r d1)
+        end
+      end
+    end.
 
-Axiom le : S -> S -> Prop.
+  Definition update_gamma (g:Gamma) (v : V) s : Gamma := 
+    fun x => if eqn x v then s else g v.
 
-Inductive assume : S -> Tm -> Gamma -> Gamma -> Prop :=
-| assume_exp s g f args b i o : lookup_Gamma g f args = (b,i,o) -> assume s (Data f args) g g
-.
+  Fixpoint assume D tm (G : Gamma) : (S * Gamma) :=
+  match tm with
+  | Code (v V) => (D, update_gamma G V (min (G V) D))
+  | Code (p P) => (G P, G)
+  | Data _ => (b Exp, G)
+  | Comb l r => 
+    match assume D l G with
+    | (arr i dl dr, G) => 
+      if incl dr D then assume dl r G
+      else (D, G)
+    | _ => (D, G)
+    end
+  end.
 
+  Fixpoint assume_output D tm (G : Gamma) : (S * Gamma) :=
+  match tm with
+  | Code (v V) => (D, update_gamma G V (min (G V) D))
+  | Code (p P) => (G P, G)
+  | Data _ => (b Exp, G)
+  | Comb l r => 
+    match assume_output D l G with
+    | (arr o dl dr, G) => 
+      if incl dr D then assume dl r G
+      else (D, G)
+    | _ => (D, G)
+    end
+  end.
+
+  Axiom infer_inputs : (seq Tm) -> S -> bool.
+  Axiom assume_outputs : (seq Tm) -> S -> Gamma * S.  
+  Axiom assume_inputs : (seq Tm) -> S -> Gamma * S.  
+
+  Axiom base_sig : program -> nat -> S.
+
+  Definition check (prog:program) atom (g:Gamma) (s:S) :=
+    match atom with
+    | Cut => (g, s)
+    | App (v V) args => 
+      let b := infer_inputs args s in
+      if b then assume_outputs args s
+      else (g, s)
+    | App (p P) args => 
+      let b := infer_inputs args s in
+      if b then assume_outputs args s
+      else (g, s)
+    end.
+
+  Axiom checks : program -> list A -> Gamma -> bool.
+
+  Definition check_entails (prog:program) (G:Gamma) (r:R) : bool :=
+    let pred := r.(pred) in
+    let args := r.(args) in
+    let premises := r.(premises) in
+    let (G', s) := assume_inputs args (prog.(sig) pred) in
+    checks prog premises G'.
+
+
+End check.
